composed invariants, client non triviality

working/composition/event_based_refinement/load_balancer/compositional/client/DistributedSystem.v.dfy
@@ -1,6 +1,118 @@
-include "../shared/DistributedSystem.t.dfy"
+include "../shared/RefinementObligation.t.dfy"
 include "Network.v.dfy"
 
-module ClientDistributedSystem refines AbstractDistributedSystem {
-    import Network = ClientNetwork
+module ClientDistributedSystem refines RefinementTheorem {
+    import opened Network = ClientNetwork
+
+    ghost predicate ValidStep(c: Constants, v: Variables, v': Variables, evt: Option<Host.Spec.Event>)
+    {
+        exists msgOps :: NextStep(c, v, v', evt, HostActionStep(0, msgOps))
+    }
+
+    ghost predicate NoOp(c: Constants, v: Variables, v': Variables)
+    {
+        exists msgOps :: NextStep(c, v, v', None, HostActionStep(0, msgOps))
+    }
+
+    ghost predicate NonTriviality_Part1Spec(c: Constants, behavior: seq<Variables>)
+    {
+        && c.WF()
+        && 0 < |behavior|
+        && Init(c, behavior[0])
+        && (forall i:nat | i < |behavior|-1 :: 
+            (|| ValidStep(c, behavior[i], behavior[i+1], None) 
+            || ValidStep(c, behavior[i], behavior[i+1], Some(Network.Host.Spec.SendRequest)) 
+            || ValidStep(c, behavior[i], behavior[i+1], Some(Network.Host.Spec.ReceiveResponse))))
+        && behavior[|behavior|-1].WF(c) 
+        && |behavior[|behavior|-1].hosts[0].requests| == 1
+    }
+
+    lemma NonTriviality_Part1(c: Constants) returns (behavior: seq<Variables>)
+        requires c.WF()
+        ensures NonTriviality_Part1Spec(c, behavior)
+    {
+        behavior := [Variables.Variables(
+            [
+                Host.Variables([], [])
+            ],
+            Network.Variables({})
+        )];
+
+        var clientReq := ServiceRequest(0, (4, 5));
+        var sent := Host.ClientRequest(clientReq);
+        var msgOps := Host.MessageOps(None, Some(sent));
+        behavior := behavior + [Variables.Variables(
+            [
+                Host.Variables([clientReq], [])
+            ],
+            Network.Variables({ sent })
+        )];
+        assert Host.SendRequest(c.hosts[0], behavior[0].hosts[0], behavior[1].hosts[0], Some(Host.Spec.SendRequest), msgOps);
+        assert NextStep(c, behavior[0], behavior[1], Some(Host.Spec.SendRequest), HostActionStep(0, msgOps));
+    }
+
+    ghost predicate ExistsCorrectClientResponse(c: Constants, part2: seq<Variables>, i: nat, request: ServiceRequest<(int, int)>)
+        requires |part2| > i + 1
+    {
+        exists msgOps :: CorrectClientResponse(c, part2, i, request, msgOps)
+    }
+
+    ghost predicate CorrectClientResponse(c: Constants, part2: seq<Variables>, i: nat, request: ServiceRequest<(int, int)>, msgOps: Host.MessageOps)
+        requires |part2| > i + 1
+    {
+        && NextStep(c, part2[i], part2[i+1], None, HostActionStep(0, msgOps)) 
+        && msgOps.send.Some?
+        && msgOps.send.value.ClientResponse?
+        && msgOps.send.value.response.seqNo == request.seqNo
+        && msgOps.send.value.response.val == request.val.0 + request.val.1
+    }
+
+    ghost predicate NonTriviality_Part2Spec(c: Constants, part1: seq<Variables>, part2: seq<Variables>)
+    {
+        && NonTriviality_Part1Spec(c, part1)
+        && |part1| < |part2|
+        && part2[0..|part1|] == part1
+        && 0 < |part2[|part1|..]|
+        && (forall i:nat | |part1| <= i < |part2| - 1 :: NoOp(c, part2[i], part2[i+1]))
+        && (forall i:nat | |part1| <= i < |part2| - 1 :: part2[i].hosts == part1[|part1|-1].hosts)
+        && (ExistsCorrectClientResponse(c, part2, |part2| - 2, part1[|part1|-1].hosts[0].requests[0]))
+    }
+
+    ghost predicate NonTriviality_Part3Spec(c: Constants, part1: seq<Variables>, part2: seq<Variables>, part3: seq<Variables>)
+    {
+        && NonTriviality_Part2Spec(c, part1, part2)
+        && |part2| < |part3|
+        && part3[0..|part2|] == part2
+        && 0 < |part3[|part2|..]|
+        && (forall i:nat | |part2| <= i < |part3|-1 :: 
+            (|| ValidStep(c, part3[i], part3[i+1], None) 
+            || ValidStep(c, part3[i], part3[i+1], Some(Network.Host.Spec.SendRequest)) 
+            || ValidStep(c, part3[i], part3[i+1], Some(Network.Host.Spec.ReceiveResponse))))
+        && part3[|part3|-1].WF(c)
+        && |part3[|part3|-1].hosts[0].responses| == 1
+        && part3[|[part3]|-1].hosts[0].responses[0].seqNo == part3[|part3|-1].hosts[0].requests[0].seqNo
+        && part3[|[part3]|-1].hosts[0].responses[0].val == part3[|part3|-1].hosts[0].requests[0].val.0 + part3[|part3|-1].hosts[0].requests[0].val.1
+    }
+
+    lemma NonTriviality_Part3(c: Constants, part1: seq<Variables>, part2: seq<Variables>) returns (behavior: seq<Variables>)
+        requires c.WF()
+        requires NonTriviality_Part2Spec(c, part1, part2)
+        ensures NonTriviality_Part3Spec(c, part1, part2, behavior)
+    {
+        behavior := part2;
+
+        var msgOps :| CorrectClientResponse(c, part2, |part2| - 2, part2[|part2|-1].hosts[0].requests[0], msgOps);
+        assert msgOps.send.Some?;
+        var recv := msgOps.send.value;
+        msgOps := Host.MessageOps(Some(recv), None);
+        var clientResp := recv.response;
+        behavior := behavior + [Variables.Variables(
+            [
+                Host.Variables(part2[|part2|-1].hosts[0].requests, [clientResp])
+            ],
+            part2[|part2|-1].network
+        )];
+        assert Host.ReceiveResponse(c.hosts[0], behavior[4].hosts[0], behavior[5].hosts[0], Some(Host.Spec.ReceiveResponse), msgOps);
+        assert NextStep(c, behavior[4], behavior[5], Some(Host.Spec.ReceiveResponse), HostActionStep(0, msgOps));
+    }
 }
