working/composition/event_based_refinement/load_balancer/compositional/abstract_composition/ComposedDistributedSystem.t.dfy
@@ -1,7 +1,7 @@
 include "../shared/Types.t.dfy"
 include "ComposedNetwork.t.dfy"
 
-// analogous to module AbstractDistributedSystem
+// analogous to module: AbstractDistributedSystem
 abstract module ComposedDistributedSystem {
     import opened Types
     import opened Network: ComposedNetwork
