working/composition/event_based_refinement/load_balancer/compositional/abstract_composition/ComposedRefinementObligation.t.dfy
@@ -1,0 +1,41 @@
+include "../shared/Types.t.dfy"
+include "ComposedDistributedSystem.t.dfy"
+
+// analogous to module: RefinementTheorem
+abstract module ComposedRefinementTheorem refines ComposedDistributedSystem {
+    //import opened Types
+    //import opened DistributedSystem: ComposedDistributedSystem
+
+    ghost function ConstantsAbstraction(c: Constants) : Spec.Constants
+        requires c.WF()
+    {
+        Spec.Constants(
+            Spec.DSA.ConstantsAbstraction(c.dsA), 
+            Spec.DSB.ConstantsAbstraction(c.dsB))
+    }
+
+    ghost function VariablesAbstraction(c: Constants, v: Variables) : Spec.Variables
+        requires v.WF(c)
+    {
+        Spec.Variables(
+            Spec.DSA.VariablesAbstraction(c.dsA, v.dsA), 
+            Spec.DSB.VariablesAbstraction(c.dsB, v.dsB))
+    }
+
+    ghost predicate Inv(c: Constants, v: Variables)
+    {
+        && Spec.DSA.Inv(c.dsA, v.dsA)
+        && Spec.DSB.Inv(c.dsB, v.dsB)
+    }
+
+    lemma RefinementInit(c: Constants, v: Variables)
+        requires Init(c, v)
+        ensures Inv(c, v)
+        ensures Spec.Init(ConstantsAbstraction(c), VariablesAbstraction(c, v))
+    
+    lemma RefinementNext(c: Constants, v: Variables, v': Variables, evt: Option<Spec.Event>, step: Step)
+        requires NextStep(c, v, v', evt, step)
+        requires Inv(c, v)
+        ensures Inv(c, v') 
+        ensures (evt.Some? && Spec.Next(ConstantsAbstraction(c), VariablesAbstraction(c, v), VariablesAbstraction(c, v'), evt.value)) || (evt.None? && VariablesAbstraction(c, v) == VariablesAbstraction(c, v'))
+}
