working/composition/event_based_refinement/load_balancer/compositional/client_server/ClientServerDistributedSystem.t.dfy
@@ -1,6 +1,0 @@
-include "../abstract_composition/ComposedDistributedSystem.t.dfy"
-include "ClientServerNetwork.t.dfy"
-
-module ClientServerDistributedSystem refines ComposedDistributedSystem {
-    import opened Network = ClientServerNetwork
-}
