working/composition/event_based_refinement/load_balancer/compositional/client_server/ClientServerDistributedSystem.v.dfy
@@ -1,0 +1,6 @@
+include "../abstract_composition/ComposedRefinementObligation.t.dfy"
+include "ClientServerNetwork.v.dfy"
+
+module ClientServerDistributedSystem refines ComposedRefinementTheorem {
+    import opened Network = ClientServerNetwork
+}
