working/composition/event_based_refinement/load_balancer/compositional/client_server/ClientServerRefinementProof.v.dfy
@@ -1,0 +1,20 @@
+include "../abstract_composition/ComposedRefinementObligation.t.dfy"
+include "ClientServerDistributedSystem.v.dfy"
+
+module ClientServerRefinementProof refines ClientServerDistributedSystem {
+    
+    lemma RefinementInit(c: Constants, v: Variables)
+//        requires DistributedSystem.Init(c, v)
+//        ensures Inv(c, v)
+//        ensures Spec.Init(ConstantsAbstraction(c), VariablesAbstraction(c, v))
+    {
+    }
+
+    lemma RefinementNext(c: Constants, v: Variables, v': Variables, evt: Option<Spec.Event>, step: Step)
+//        requires DistributedSystem.NextStep(c, v, v', evt, step)
+//        requires Inv(c, v)
+//        ensures Inv(c, v') 
+//        ensures Spec.Next(ConstantsAbstraction(c), VariablesAbstraction(c, v), VariablesAbstraction(c, v'), evt) || (VariablesAbstraction(c, v) == VariablesAbstraction(c, v') && evt == NoOp)
+    {
+    }
+}
