working/composition/event_based_refinement/load_balancer/compositional/server/DistributedSystem.v.dfy
@@ -1,6 +1,7 @@
 include "../shared/DistributedSystem.t.dfy"
+include "../shared/RefinementObligation.t.dfy"
 include "Network.v.dfy"
 
-module ServerDistributedSystem refines AbstractDistributedSystem {
-    import Network = ServerNetwork
+module ServerDistributedSystem refines RefinementTheorem {
+    import opened Network = ServerNetwork
 }
